U -> D

fstar/MLS.Tree.Lemmas.fst
@@ -8,38 +8,38 @@ let lemma_mult_lt_right_inv (a:int) (b:int) (c:nat): Lemma (requires a*c < b*c) 
 
 #set-options "--fuel 1 --ifuel 0 --z3cliopt smt.arith.nl=false"
 
-val leaf_index_inside_right_index: lu:pos -> lp:nat{lu <= lp} -> iu:tree_index lu -> ip:tree_index lp -> Lemma
-  (requires leaf_index_inside lp ip iu)
-  (ensures leaf_index_inside lp ip (right_index iu))
-  [SMTPat (leaf_index_inside lp ip (right_index iu))]
-let leaf_index_inside_right_index lu lp iu ip =
+val leaf_index_inside_right_index: ld:pos -> lp:nat{ld <= lp} -> id:tree_index ld -> ip:tree_index lp -> Lemma
+  (requires leaf_index_inside lp ip id)
+  (ensures leaf_index_inside lp ip (right_index id))
+  [SMTPat (leaf_index_inside lp ip (right_index id))]
+let leaf_index_inside_right_index ld lp id ip =
   let open FStar.Math.Lemmas in
-  eliminate exists ku kp. (iu == ku*(pow2 lu)) /\ (ip == kp*(pow2 lp))
-  returns (iu + pow2 (lu - 1) < ip + pow2 lp)
+  eliminate exists ku kp. (id == ku*(pow2 ld)) /\ (ip == kp*(pow2 lp))
+  returns (id + pow2 (ld - 1) < ip + pow2 lp)
   with _. (
     FStar.Math.Lemmas.distributivity_add_left kp 1 (pow2 lp);
-    FStar.Math.Lemmas.pow2_plus lu (lp-lu);
-    FStar.Math.Lemmas.paren_mul_right (kp+1) (pow2 (lp-lu)) (pow2 lu);
-    lemma_mult_lt_right_inv ku ((kp+1)*(pow2 (lp-lu))) (pow2 lu);
-    FStar.Math.Lemmas.lemma_mult_le_right (pow2 lu) (ku+1) ((kp+1) * (pow2 (lp-lu)));
-    FStar.Math.Lemmas.distributivity_add_left ku 1 (pow2 lu)
+    FStar.Math.Lemmas.pow2_plus ld (lp-ld);
+    FStar.Math.Lemmas.paren_mul_right (kp+1) (pow2 (lp-ld)) (pow2 ld);
+    lemma_mult_lt_right_inv ku ((kp+1)*(pow2 (lp-ld))) (pow2 ld);
+    FStar.Math.Lemmas.lemma_mult_le_right (pow2 ld) (ku+1) ((kp+1) * (pow2 (lp-ld)));
+    FStar.Math.Lemmas.distributivity_add_left ku 1 (pow2 ld)
   )
 
-val leaf_index_same_side: lu:nat -> lp:nat{lu < lp} -> iu:tree_index lu -> ip:tree_index lp{leaf_index_inside lp ip iu} -> li:leaf_index lp ip -> Lemma
-  (requires lu < lp /\ leaf_index_inside lp ip iu /\ leaf_index_inside lu iu li)
-  (ensures is_left_leaf #lp #ip iu <==> is_left_leaf #lp #ip li)
-let leaf_index_same_side lu lp iu ip li =
-  if is_left_leaf #lp #ip iu then (
-    eliminate exists ku kp. iu = ku*(pow2 lu) /\ ip = kp*(pow2 lp)
+val leaf_index_same_side: ld:nat -> lp:nat{ld < lp} -> id:tree_index ld -> ip:tree_index lp{leaf_index_inside lp ip id} -> li:leaf_index lp ip -> Lemma
+  (requires ld < lp /\ leaf_index_inside lp ip id /\ leaf_index_inside ld id li)
+  (ensures is_left_leaf #lp #ip id <==> is_left_leaf #lp #ip li)
+let leaf_index_same_side ld lp id ip li =
+  if is_left_leaf #lp #ip id then (
+    eliminate exists ku kp. id = ku*(pow2 ld) /\ ip = kp*(pow2 lp)
     returns (li < ip+(pow2 (lp-1)))
     with _. (
       FStar.Math.Lemmas.paren_mul_right kp 2 (pow2 (lp-1));
       FStar.Math.Lemmas.distributivity_add_left (kp*2) 1 (pow2 (lp-1));
-      FStar.Math.Lemmas.pow2_plus (lp-1-lu) lu;
-      FStar.Math.Lemmas.paren_mul_right (kp*2+1) (pow2 (lp-1-lu)) (pow2 lu);
-      lemma_mult_lt_right_inv ku ((2*kp+1)*(pow2 (lp-1-lu))) (pow2 lu);
-      FStar.Math.Lemmas.lemma_mult_le_right (pow2 lu) (ku+1) ((2*kp+1)*(pow2 (lp-1-lu)));
-      FStar.Math.Lemmas.distributivity_add_left ku 1 (pow2 lu)
+      FStar.Math.Lemmas.pow2_plus (lp-1-ld) ld;
+      FStar.Math.Lemmas.paren_mul_right (kp*2+1) (pow2 (lp-1-ld)) (pow2 ld);
+      lemma_mult_lt_right_inv ku ((2*kp+1)*(pow2 (lp-1-ld))) (pow2 ld);
+      FStar.Math.Lemmas.lemma_mult_le_right (pow2 ld) (ku+1) ((2*kp+1)*(pow2 (lp-1-ld)));
+      FStar.Math.Lemmas.distributivity_add_left ku 1 (pow2 ld)
     )
   ) else ()
 
@@ -62,19 +62,19 @@ let left_right_index_disj #l1 #l2 i1 i2 =
   )
 
 val leaf_index_inside_subtree:
-  lu:nat -> lc:nat{lu <= lc} -> iu:tree_index lu -> ic:tree_index lc -> li:leaf_index lu iu -> Lemma
-  (requires leaf_index_inside lc ic iu)
+  ld:nat -> lc:nat{ld <= lc} -> id:tree_index ld -> ic:tree_index lc -> li:leaf_index ld id -> Lemma
+  (requires leaf_index_inside lc ic id)
   (ensures leaf_index_inside lc ic li)
-let leaf_index_inside_subtree lu lc iu ic li =
-  eliminate exists ku kc. (iu == ku*(pow2 lu)) /\ (ic == kc*(pow2 lc))
+let leaf_index_inside_subtree ld lc id ic li =
+  eliminate exists ku kc. (id == ku*(pow2 ld)) /\ (ic == kc*(pow2 lc))
   returns (li < ic + pow2 lc)
   with _. (
-    FStar.Math.Lemmas.pow2_plus (lc-lu) lu;
+    FStar.Math.Lemmas.pow2_plus (lc-ld) ld;
     FStar.Math.Lemmas.distributivity_add_left kc 1 (pow2 lc);
-    FStar.Math.Lemmas.paren_mul_right (kc+1) (pow2 (lc-lu)) (pow2 lu);
-    lemma_mult_lt_right_inv ku ((kc+1) * (pow2 (lc-lu))) (pow2 lu);
-    FStar.Math.Lemmas.lemma_mult_le_right (pow2 lu) (ku+1) ((kc+1) * (pow2 (lc-lu)));
-    FStar.Math.Lemmas.distributivity_add_left ku 1 (pow2 lu)
+    FStar.Math.Lemmas.paren_mul_right (kc+1) (pow2 (lc-ld)) (pow2 ld);
+    lemma_mult_lt_right_inv ku ((kc+1) * (pow2 (lc-ld))) (pow2 ld);
+    FStar.Math.Lemmas.lemma_mult_le_right (pow2 ld) (ku+1) ((kc+1) * (pow2 (lc-ld)));
+    FStar.Math.Lemmas.distributivity_add_left ku 1 (pow2 ld)
   )
 
 #set-options "--fuel 1 --ifuel 1"
